yet more progress

compiler1/proofs/lab_to_targetProofScript.sml
@@ -58,8 +58,145 @@ in
     \\ TRY (Cases_on `r`)
     \\ EVAL_TAC \\ fs [] \\ rw []
     \\ CONV_TAC (DEPTH_CONV PairRules.PBETA_CONV)
-    \\ fs [SND_read_mem_word,write_mem_word_consts])
+    \\ fs [SND_read_mem_word_consts,write_mem_word_consts])
 end
+
+(* -- *)
+
+val enc_with_nop_def = Define `
+  enc_with_nop enc (b:'a asm) bytes =
+    ?n. bytes = enc b ++ FLAT (REPLICATE n (enc (asm$Inst Skip)))`
+
+val asm_step_nop_def = Define `
+  asm_step_nop enc bytes c s1 i s2 <=>
+    bytes_in_memory s1.pc bytes s1.mem s1.mem_domain /\
+    enc_with_nop enc i bytes /\
+    (case c.link_reg of NONE => T | SOME r => s1.lr = r) /\
+    (s1.be <=> c.big_endian) /\ s1.align = c.code_alignment /\
+    asm i (s1.pc + n2w (LENGTH bytes)) s1 = s2 /\ ~s2.failed /\
+    asm_ok i c`
+
+val evaluate_nop_step =
+  asm_step_IMP_evaluate_step
+    |> SIMP_RULE std_ss [asm_step_alt_def]
+    |> SPEC_ALL |> Q.INST [`i`|->`Inst Skip`]
+    |> SIMP_RULE (srw_ss()) [asm_def,inst_def,asm_ok_def,inst_ok_def,
+         Once upd_pc_def,GSYM CONJ_ASSOC]
+
+val shift_interfer_0 = prove(
+  ``shift_interfer 0 = I``,
+  fs [shift_interfer_def,FUN_EQ_THM,shift_seq_def,
+      machine_config_component_equality]);
+
+val upd_pc_with_pc = prove(
+  ``upd_pc s1.pc s1 = s1:'a asm_state``,
+  fs [asm_state_component_equality,upd_pc_def]);
+
+val shift_interfer_twice = store_thm("shift_interfer_twice[simp]",
+  ``shift_interfer l' (shift_interfer l c) =
+    shift_interfer (l + l') c``,
+  fs [shift_interfer_def,shift_seq_def,AC ADD_COMM ADD_ASSOC]);
+
+val evaluate_nop_steps = prove(
+  ``!n s1 ms1 c.
+      backend_correct_alt c.f c.asm_config /\
+      c.prog_addresses = s1.mem_domain /\
+      interference_ok c.next_interfer (c.f.proj s1.mem_domain) /\
+      bytes_in_memory s1.pc (FLAT (REPLICATE n (c.f.encode (Inst Skip)))) s1.mem
+        s1.mem_domain /\
+      (case c.asm_config.link_reg of NONE => T | SOME r => s1.lr = r) /\
+      (s1.be <=> c.asm_config.big_endian) /\
+      s1.align = c.asm_config.code_alignment /\ ~s1.failed /\
+      c.f.state_rel (s1:'a asm_state) (ms1:'state) ==>
+      ?l ms2.
+        !k.
+          evaluate c io (k + l) ms1 =
+          evaluate (shift_interfer l c) io k ms2 /\
+          c.f.state_rel
+            (upd_pc (s1.pc + n2w (n * LENGTH (c.f.encode (Inst Skip)))) s1)
+            ms2``,
+  Induct \\ fs [] THEN1
+   (rpt strip_tac \\ Q.LIST_EXISTS_TAC [`0`,`ms1`]
+    \\ fs [shift_interfer_0,upd_pc_with_pc])
+  \\ rpt strip_tac \\ fs [REPLICATE,bytes_in_memory_APPEND]
+  \\ mp_tac evaluate_nop_step \\ fs [] \\ rpt strip_tac
+  \\ fs [GSYM PULL_FORALL]
+  \\ first_x_assum (mp_tac o
+       Q.SPECL [`(upd_pc (s1.pc +
+          n2w (LENGTH ((c:('a,'state,'b) machine_config).f.encode
+            (Inst Skip)))) s1)`,`ms2`,`shift_interfer l c`])
+  \\ match_mp_tac IMP_IMP \\ strip_tac
+  THEN1 (fs [shift_interfer_def,upd_pc_def,interference_ok_def,shift_seq_def])
+  \\ rpt strip_tac
+  \\ `(shift_interfer l c).f = c.f` by fs [shift_interfer_def]
+  \\ fs [upd_pc_def]
+  \\ Q.LIST_EXISTS_TAC [`l'+l`,`ms2'`]
+  \\ full_simp_tac std_ss [GSYM WORD_ADD_ASSOC,
+       word_add_n2w,AC ADD_COMM ADD_ASSOC,MULT_CLAUSES]
+  \\ fs [ADD_ASSOC] \\ rpt strip_tac
+  \\ first_x_assum (mp_tac o Q.SPEC `k`)
+  \\ first_x_assum (mp_tac o Q.SPEC `k+l'`)
+  \\ fs [AC ADD_COMM ADD_ASSOC]);
+
+val asm_step_IMP_evaluate_step_nop = prove(
+  ``!c s1 ms1 io i s2 bytes.
+      backend_correct_alt c.f c.asm_config /\
+      c.prog_addresses = s1.mem_domain /\
+      interference_ok c.next_interfer (c.f.proj s1.mem_domain) /\
+      bytes_in_memory s1.pc bytes s2.mem s1.mem_domain /\
+      asm_step_nop c.f.encode bytes c.asm_config s1 i s2 /\
+      s2 = asm i (s1.pc + n2w (LENGTH bytes)) s1 /\
+      c.f.state_rel (s1:'a asm_state) (ms1:'state) /\
+      (!x. i <> Call x) ==>
+      ?l ms2.
+        !k.
+          evaluate c io (k + l) ms1 =
+          evaluate (shift_interfer l c) io k ms2 /\
+          c.f.state_rel s2 ms2 /\ l <> 0``,
+  fs [asm_step_nop_def] \\ rpt strip_tac
+  \\ (asm_step_IMP_evaluate_step
+      |> SIMP_RULE std_ss [asm_step_alt_def] |> SPEC_ALL |> mp_tac) \\ fs []
+  \\ fs [enc_with_nop_def]
+  \\ match_mp_tac IMP_IMP \\ strip_tac THEN1
+   (fs [bytes_in_memory_APPEND] \\ Cases_on `i`
+    \\ fs [asm_def,upd_pc_def,jump_to_offset_def,upd_reg_def,
+           LET_DEF,assert_def] \\ rw [] \\ fs [] \\ rfs [])
+  \\ rpt strip_tac \\ fs [GSYM PULL_FORALL]
+  \\ Cases_on `?w. i = Jump w` \\ fs []
+  THEN1 (fs [asm_def] \\ Q.LIST_EXISTS_TAC [`l`,`ms2`] \\ fs [])
+  \\ Cases_on `?c n r w. (i = JumpCmp c n r w) /\
+                  word_cmp c (read_reg n s1) (reg_imm r s1)` \\ fs []
+  THEN1 (rw [] \\ fs [asm_def] \\ Q.LIST_EXISTS_TAC [`l`,`ms2`] \\ fs [])
+  \\ Cases_on `?r. (i = JumpReg r)` \\ fs []
+  THEN1 (rw [] \\ fs [asm_def,LET_DEF] \\ Q.LIST_EXISTS_TAC [`l`,`ms2`]
+               \\ fs [] \\ rfs [])
+  \\ qspecl_then [`n`,`asm i (s1.pc + n2w (LENGTH (c.f.encode i))) s1`,`ms2`,
+       `shift_interfer l c`] mp_tac evaluate_nop_steps
+  \\ match_mp_tac IMP_IMP \\ strip_tac
+  THEN1 (fs [shift_interfer_def] \\ rpt strip_tac
+    THEN1 (fs [interference_ok_def,shift_seq_def])
+    THEN1
+     (Q.ABBREV_TAC `mm = (asm i (s1.pc + n2w (LENGTH (c.f.encode i))) s1).mem`
+      \\ fs [Once (asm_mem_ignore_new_pc |> Q.SPECL [`i`,`0w`])]
+      \\ `!w. (asm i w s1).pc = w` by (Cases_on `i` \\ fs [asm_def,upd_pc_def])
+      \\ fs [bytes_in_memory_APPEND])
+    \\ metis_tac [asm_failed_ignore_new_pc])
+  \\ rpt strip_tac \\ fs [GSYM PULL_FORALL]
+  \\ Q.LIST_EXISTS_TAC [`l+l'`,`ms2'`]
+  \\ fs [PULL_FORALL] \\ strip_tac
+  \\ first_x_assum (mp_tac o Q.SPEC `k:num`)
+  \\ qpat_assum `!k. xx = yy` (mp_tac o Q.SPEC `k+l':num`)
+  \\ rpt strip_tac \\ fs [AC ADD_COMM ADD_ASSOC]
+  \\ fs [shift_interfer_def]
+  \\ qpat_assum `c.f.state_rel xx yy` mp_tac
+  \\ match_mp_tac (METIS_PROVE [] ``(x = z) ==> (f x y ==> f z y)``)
+  \\ Cases_on `i` \\ fs [asm_def]
+  \\ fs [LENGTH_FLAT,SUM_REPLICATE,map_replicate]
+  \\ full_simp_tac std_ss [GSYM WORD_ADD_ASSOC,word_add_n2w]
+  THEN1 (Cases_on `i'` \\ fs [inst_def,upd_pc_def]
+    \\ full_simp_tac std_ss [GSYM WORD_ADD_ASSOC,word_add_n2w])
+  \\ fs [jump_to_offset_def,upd_pc_def]
+  \\ full_simp_tac std_ss [GSYM WORD_ADD_ASSOC,word_add_n2w]);
 
 (* -- *)
 
@@ -92,9 +229,17 @@ val option_ldrop_lemma = prove(
 
 val IMP_IMP2 = METIS_PROVE [] ``a /\ (a /\ b ==> c) ==> ((a ==> b) ==> c)``
 
-val enc_with_nop_def = Define `
-  enc_with_nop enc (b:'a asm) bytes =
-    ?n. bytes = enc b ++ FLAT (REPLICATE n (enc (asm$Inst Skip)))`
+val lab_lookup_def = Define `
+  lab_lookup k1 k2 labs =
+    case lookup k1 labs of
+    | NONE => NONE
+    | SOME f => lookup k2 f`
+
+val lab_lookup_IMP = prove(
+  ``(lab_lookup l1 l2 labs = SOME x) ==>
+    (find_pos (Lab l1 l2) labs = x)``,
+  fs [lab_lookup_def,find_pos_def,lookup_any_def]
+  \\ BasicProvers.EVERY_CASE_TAC);
 
 val line_ok_def = Define `
   (line_ok (c:'a asm_config) enc labs pos (Label _ _ l) <=>
@@ -119,7 +264,8 @@ val line_ok_def = Define `
      let target = find_pos (get_label a) labs in
      let w1 = n2w target - n2w pos in
        enc_with_nop enc (lab_inst w1 a) bytes /\
-       (LENGTH bytes = l) /\ asm_ok (lab_inst w1 a) c)`
+       (LENGTH bytes = l) /\ asm_ok (lab_inst w1 a) c /\
+       (case get_label a of Lab l1 l2 => (lab_lookup l1 l2 labs <> NONE)))`
 
 val all_enc_ok_def = Define `
   (all_enc_ok c enc labs pos [] = T) /\
@@ -147,18 +293,6 @@ val code_similar_def = Define `
      code_similar rest1 rest2 /\
      EVERY2 line_similar lines1 lines2 /\ (s1 = s2)) /\
   (code_similar _ _ = F)`
-
-val lab_lookup_def = Define `
-  lab_lookup k1 k2 labs =
-    case lookup k1 labs of
-    | NONE => NONE
-    | SOME f => lookup k2 f`
-
-val lab_lookup_IMP = prove(
-  ``(lab_lookup l1 l2 labs = SOME x) ==>
-    (find_pos (Lab l1 l2) labs = x)``,
-  fs [lab_lookup_def,find_pos_def,lookup_any_def]
-  \\ BasicProvers.EVERY_CASE_TAC);
 
 val word_loc_val_def = Define `
   (word_loc_val p labs (Word w) = SOME w) /\
@@ -393,7 +527,7 @@ val IMP_bytes_in_memory_Call = prove(
     bytes_in_memory p (prog_to_bytes mc_conf.f.encode code2) t1.mem
       (t1:'a asm_state).mem_domain /\
     (asm_fetch s1 = SOME (LabAsm (Call ww) l bytes n)) ==>
-    (1 = 2)``,
+    F``,
   rpt strip_tac
   \\ fs [asm_fetch_def,LET_DEF]
   \\ imp_res_tac IMP_bytes_in_memory
@@ -406,23 +540,28 @@ val IMP_bytes_in_memory_LocValue = prove(
     bytes_in_memory p (prog_to_bytes mc_conf.f.encode code2) t1.mem
       t1.mem_domain /\
     (asm_fetch s1 = SOME (LabAsm (LocValue reg (Lab l1 l2)) l bytes n)) ==>
-    ?tt enc.
+    ?tt bytes.
       (tt = n2w (find_pos (Lab l1 l2) labs) -
             n2w (pos_val s1.pc 0 code2)) /\
-      (enc = mc_conf.f.encode (Loc reg tt)) /\
+      enc_with_nop mc_conf.f.encode (Loc reg tt) bytes /\
       bytes_in_memory ((p:'a word) + n2w (pos_val s1.pc 0 code2))
-        enc t1.mem t1.mem_domain /\
-      asm_ok (Loc reg tt) (mc_conf: ('a,'state,'b) machine_config).asm_config``,
+        bytes t1.mem t1.mem_domain /\
+      (pos_val (s1.pc+1) 0 code2 = pos_val s1.pc 0 code2 + LENGTH bytes) /\
+      asm_ok (Loc reg tt) (mc_conf: ('a,'state,'b) machine_config).asm_config /\
+      lab_lookup l1 l2 labs <> NONE``,
   fs [asm_fetch_def,LET_DEF]
   \\ Q.SPEC_TAC (`s1.pc`,`pc`) \\ strip_tac
   \\ Q.SPEC_TAC (`s1.code`,`code1`) \\ strip_tac \\ strip_tac
   \\ mp_tac (IMP_bytes_in_memory |> Q.GENL [`i`,`dm`,`m`]) \\ fs []
   \\ strip_tac \\ res_tac
   \\ Cases_on `j` \\ fs [line_similar_def] \\ rw []
-  \\ fs [line_ok_def,enc_with_nop_def,LET_DEF] \\ rw []
+  \\ fs [line_ok_def,LET_DEF] \\ rw []
+  \\ Q.EXISTS_TAC `l'` \\ fs [enc_with_nop_def,PULL_EXISTS]
+  \\ qexists_tac `n'` \\ fs []
   \\ fs [no_Label_eq,LET_DEF,lab_inst_def,get_label_def] \\ rw []
   \\ fs [asm_fetch_aux_def,all_bytes_def,LET_DEF,line_bytes_def,
-         bytes_in_memory_APPEND]);
+         bytes_in_memory_APPEND] \\ rw []
+  \\ cheat);
 
 val IMP_bytes_in_memory_CallFFI = prove(
   ``code_similar s1.code code2 /\
@@ -738,7 +877,6 @@ val compile_correct = Q.prove(
     \\ Q.EXISTS_TAC `k + l' - 1` \\ fs []
     \\ Q.EXISTS_TAC `t2` \\ fs [state_rel_def,shift_interfer_def])
   THEN1 (* JumpCmp *) cheat
-
   THEN1 (* Call *)
    (qmatch_assum_rename_tac
          `asm_fetch s1 = SOME (LabAsm (Call lab) x1 x2 x3)`
@@ -747,11 +885,9 @@ val compile_correct = Q.prove(
          `asm_fetch s1 = SOME (LabAsm (Call (Lab l1 l2)) l bytes len)`
     \\ mp_tac (Q.INST [`ww`|->`Lab l1 l2`,`n`|->`len`]
             IMP_bytes_in_memory_Call)
-    \\ match_mp_tac IMP_IMP \\ strip_tac
-    THEN1 (fs [state_rel_def] \\ imp_res_tac bytes_in_mem_IMP \\ fs [])
-    \\ fs [])
+    \\ match_mp_tac IMP_IMP \\ strip_tac \\ fs []
+    \\ fs [state_rel_def] \\ imp_res_tac bytes_in_mem_IMP \\ fs [])
   THEN1 (* LocValue *)
-
    (qmatch_assum_rename_tac
          `asm_fetch s1 = SOME (LabAsm (LocValue reg lab) x1 x2 x3)`
     \\ Cases_on `lab`
@@ -762,19 +898,19 @@ val compile_correct = Q.prove(
                IMP_bytes_in_memory_LocValue) \\ fs []
     \\ match_mp_tac IMP_IMP \\ strip_tac
     THEN1 (fs [state_rel_def] \\ imp_res_tac bytes_in_mem_IMP \\ fs [])
-    \\ rpt strip_tac \\ pop_assum mp_tac
+    \\ rpt strip_tac \\ pop_assum mp_tac \\ pop_assum mp_tac
     \\ qpat_abbrev_tac `jj = asm$Loc reg lll` \\ rpt strip_tac
     \\ MP_TAC (Q.SPECL [`mc_conf`,`t1`,`ms1`,`s1.io_events`,`jj`]
-         asm_step_IMP_evaluate_step) \\ fs []
+         asm_step_IMP_evaluate_step_nop) \\ fs []
+    \\ strip_tac \\ pop_assum (mp_tac o Q.SPEC `bytes'`)
     \\ MATCH_MP_TAC IMP_IMP \\ STRIP_TAC THEN1
-     (fs [state_rel_def,asm_def,LET_DEF]
-      \\ fs [asm_step_alt_def,asm_def,LET_DEF]
-      \\ imp_res_tac bytes_in_mem_IMP
-      \\ unabbrev_all_tac \\ fs [asm_def,upd_pc_def,upd_reg_def])
+     (fs [state_rel_def,asm_def,LET_DEF] \\ unabbrev_all_tac \\ fs []
+      \\ fs [asm_step_nop_def,asm_def,LET_DEF]
+      \\ fs [asm_def,upd_pc_def,upd_reg_def])
     \\ rpt strip_tac
-    \\ FIRST_X_ASSUM (MP_TAC o Q.SPECL [`shift_interfer l' mc_conf`,
+    \\ FIRST_X_ASSUM (MP_TAC o Q.SPECL [`shift_interfer l mc_conf`,
          `code2`,`labs`,
-         `(asm jj (t1.pc + n2w (LENGTH (mc_conf.f.encode jj))) t1)`,`ms2`])
+         `(asm jj (t1.pc + n2w (LENGTH (bytes':word8 list))) t1)`,`ms2`])
     \\ MATCH_MP_TAC IMP_IMP \\ STRIP_TAC THEN1
      (unabbrev_all_tac
       \\ fs [shift_interfer_def,state_rel_def,asm_def,LET_DEF] \\ rfs[]
@@ -786,13 +922,14 @@ val compile_correct = Q.prove(
       \\ fs [interference_ok_def,shift_seq_def,read_reg_def]
       \\ rewrite_tac [GSYM word_add_n2w,GSYM word_sub_def,WORD_SUB_PLUS,
             WORD_ADD_SUB] \\ fs [get_pc_value_def]
-      \\ cheat)
+      \\ fs [APPLY_UPDATE_THM] \\ rw [word_loc_val_def]
+      \\ Cases_on `lab_lookup l1 l2 labs` \\ fs []
+      \\ imp_res_tac lab_lookup_IMP \\ rw [])
+    \\ rpt strip_tac \\ fs [inc_pc_def,dec_clock_def,labSemTheory.upd_reg_def]
+    \\ FIRST_X_ASSUM (MP_TAC o Q.SPEC `s1.clock - 1 + k`)
     \\ rpt strip_tac
-    \\ FIRST_X_ASSUM (MP_TAC o Q.SPEC `s1.clock - 1 + k`) \\ rw []
-    \\ `s1.clock - 1 + k + l = s1.clock + (k + l - 1)` by DECIDE_TAC
     \\ Q.EXISTS_TAC `k + l - 1` \\ fs []
-    \\ Q.EXISTS_TAC `t2` \\ fs [state_rel_def,shift_interfer_def] \\ cheat)
-
+    \\ `s1.clock - 1 + k + l = s1.clock + (k + l - 1)` by decide_tac \\ fs [])
   THEN1 (* CallFFI *)
    (qmatch_assum_rename_tac `asm_fetch s1 = SOME (LabAsm (CallFFI n') l1 l2 l3)`
     \\ qmatch_assum_rename_tac
@@ -967,140 +1104,10 @@ val compile_correct = Q.prove(
 (*
 
 TODO:
+ - force all labels to have length 0, and no padding at the end of sections
  - define an incremental version of the compiler
  - add ability to install code
 
 *)
-
-val asm_step_nop_def = Define `
-  asm_step_nop enc bytes c s1 i s2 <=>
-    bytes_in_memory s1.pc bytes s1.mem s1.mem_domain /\
-    enc_with_nop enc i bytes /\
-    (case c.link_reg of NONE => T | SOME r => s1.lr = r) /\
-    (s1.be <=> c.big_endian) /\ s1.align = c.code_alignment /\
-    asm i (s1.pc + n2w (LENGTH bytes)) s1 = s2 /\ ~s2.failed /\
-    asm_ok i c`
-
-val evaluate_nop_step =
-  asm_step_IMP_evaluate_step
-    |> SIMP_RULE std_ss [asm_step_alt_def]
-    |> SPEC_ALL |> Q.INST [`i`|->`Inst Skip`]
-    |> SIMP_RULE (srw_ss()) [asm_def,inst_def,asm_ok_def,inst_ok_def,
-         Once upd_pc_def,GSYM CONJ_ASSOC]
-
-val shift_interfer_0 = prove(
-  ``shift_interfer 0 = I``,
-  fs [shift_interfer_def,FUN_EQ_THM,shift_seq_def,
-      machine_config_component_equality]);
-
-val upd_pc_with_pc = prove(
-  ``upd_pc s1.pc s1 = s1:'a asm_state``,
-  fs [asm_state_component_equality,upd_pc_def]);
-
-val shift_interfer_twice = store_thm("shift_interfer_twice[simp]",
-  ``shift_interfer l' (shift_interfer l c) =
-    shift_interfer (l + l') c``,
-  fs [shift_interfer_def,shift_seq_def,AC ADD_COMM ADD_ASSOC]);
-
-val evaluate_nop_steps = prove(
-  ``!n s1 ms1 c.
-      backend_correct_alt c.f c.asm_config /\
-      c.prog_addresses = s1.mem_domain /\
-      interference_ok c.next_interfer (c.f.proj s1.mem_domain) /\
-      bytes_in_memory s1.pc (FLAT (REPLICATE n (c.f.encode (Inst Skip)))) s1.mem
-        s1.mem_domain /\
-      (case c.asm_config.link_reg of NONE => T | SOME r => s1.lr = r) /\
-      (s1.be <=> c.asm_config.big_endian) /\
-      s1.align = c.asm_config.code_alignment /\ ~s1.failed /\
-      c.f.state_rel (s1:'a asm_state) (ms1:'state) ==>
-      ?l ms2.
-        !k.
-          evaluate c io (k + l) ms1 =
-          evaluate (shift_interfer l c) io k ms2 /\
-          c.f.state_rel
-            (upd_pc (s1.pc + n2w (n * LENGTH (c.f.encode (Inst Skip)))) s1)
-            ms2``,
-  Induct \\ fs [] THEN1
-   (rpt strip_tac \\ Q.LIST_EXISTS_TAC [`0`,`ms1`]
-    \\ fs [shift_interfer_0,upd_pc_with_pc])
-  \\ rpt strip_tac \\ fs [REPLICATE,bytes_in_memory_APPEND]
-  \\ mp_tac evaluate_nop_step \\ fs [] \\ rpt strip_tac
-  \\ fs [GSYM PULL_FORALL]
-  \\ first_x_assum (mp_tac o
-       Q.SPECL [`(upd_pc (s1.pc +
-          n2w (LENGTH ((c:('a,'state,'b) machine_config).f.encode
-            (Inst Skip)))) s1)`,`ms2`,`shift_interfer l c`])
-  \\ match_mp_tac IMP_IMP \\ strip_tac
-  THEN1 (fs [shift_interfer_def,upd_pc_def,interference_ok_def,shift_seq_def])
-  \\ rpt strip_tac
-  \\ `(shift_interfer l c).f = c.f` by fs [shift_interfer_def]
-  \\ fs [upd_pc_def]
-  \\ Q.LIST_EXISTS_TAC [`l'+l`,`ms2'`]
-  \\ full_simp_tac std_ss [GSYM WORD_ADD_ASSOC,
-       word_add_n2w,AC ADD_COMM ADD_ASSOC,MULT_CLAUSES]
-  \\ fs [ADD_ASSOC] \\ rpt strip_tac
-  \\ first_x_assum (mp_tac o Q.SPEC `k`)
-  \\ first_x_assum (mp_tac o Q.SPEC `k+l'`)
-  \\ fs [AC ADD_COMM ADD_ASSOC]);
-
-val asm_step_IMP_evaluate_step_nop = prove(
-  ``!c s1 ms1 io i s2 bytes.
-      backend_correct_alt c.f c.asm_config /\
-      c.prog_addresses = s1.mem_domain /\
-      interference_ok c.next_interfer (c.f.proj s1.mem_domain) /\
-      bytes_in_memory s1.pc bytes s2.mem s1.mem_domain /\
-      asm_step_nop c.f.encode bytes c.asm_config s1 i s2 /\
-      s2 = asm i (s1.pc + n2w (LENGTH bytes)) s1 /\
-      c.f.state_rel (s1:'a asm_state) (ms1:'state) /\
-      (!x. i <> Call x) ==>
-      ?l ms2.
-        !k.
-          evaluate c io (k + l) ms1 =
-          evaluate (shift_interfer l c) io k ms2 /\
-          c.f.state_rel s2 ms2 /\ l <> 0``,
-  fs [asm_step_nop_def] \\ rpt strip_tac
-  \\ (asm_step_IMP_evaluate_step
-      |> SIMP_RULE std_ss [asm_step_alt_def] |> SPEC_ALL |> mp_tac) \\ fs []
-  \\ fs [enc_with_nop_def]
-  \\ match_mp_tac IMP_IMP \\ strip_tac THEN1
-   (fs [bytes_in_memory_APPEND] \\ Cases_on `i`
-    \\ fs [asm_def,upd_pc_def,jump_to_offset_def,upd_reg_def,
-           LET_DEF,assert_def] \\ rw [] \\ fs [] \\ rfs [])
-  \\ rpt strip_tac \\ fs [GSYM PULL_FORALL]
-  \\ Cases_on `?w. i = Jump w` \\ fs []
-  THEN1 (fs [asm_def] \\ Q.LIST_EXISTS_TAC [`l`,`ms2`] \\ fs [])
-  \\ Cases_on `?c n r w. (i = JumpCmp c n r w) /\
-                  word_cmp c (read_reg n s1) (reg_imm r s1)` \\ fs []
-  THEN1 (rw [] \\ fs [asm_def] \\ Q.LIST_EXISTS_TAC [`l`,`ms2`] \\ fs [])
-  \\ Cases_on `?r. (i = JumpReg r)` \\ fs []
-  THEN1 (rw [] \\ fs [asm_def,LET_DEF] \\ Q.LIST_EXISTS_TAC [`l`,`ms2`]
-               \\ fs [] \\ rfs [])
-  \\ qspecl_then [`n`,`asm i (s1.pc + n2w (LENGTH (c.f.encode i))) s1`,`ms2`,
-       `shift_interfer l c`] mp_tac evaluate_nop_steps
-  \\ match_mp_tac IMP_IMP \\ strip_tac
-  THEN1 (fs [shift_interfer_def] \\ rpt strip_tac
-    THEN1 (fs [interference_ok_def,shift_seq_def])
-    THEN1
-     (Q.ABBREV_TAC `mm = (asm i (s1.pc + n2w (LENGTH (c.f.encode i))) s1).mem`
-      \\ fs [Once (asm_mem_ignore_new_pc |> Q.SPECL [`i`,`0w`])]
-      \\ `!w. (asm i w s1).pc = w` by (Cases_on `i` \\ fs [asm_def,upd_pc_def])
-      \\ fs [bytes_in_memory_APPEND])
-    \\ metis_tac [asm_failed_ignore_new_pc])
-  \\ rpt strip_tac \\ fs [GSYM PULL_FORALL]
-  \\ Q.LIST_EXISTS_TAC [`l+l'`,`ms2'`]
-  \\ fs [PULL_FORALL] \\ strip_tac
-  \\ first_x_assum (mp_tac o Q.SPEC `k:num`)
-  \\ qpat_assum `!k. xx = yy` (mp_tac o Q.SPEC `k+l':num`)
-  \\ rpt strip_tac \\ fs [AC ADD_COMM ADD_ASSOC]
-  \\ fs [shift_interfer_def]
-  \\ qpat_assum `c.f.state_rel xx yy` mp_tac
-  \\ match_mp_tac (METIS_PROVE [] ``(x = z) ==> (f x y ==> f z y)``)
-  \\ Cases_on `i` \\ fs [asm_def]
-  \\ fs [LENGTH_FLAT,SUM_REPLICATE,map_replicate]
-  \\ full_simp_tac std_ss [GSYM WORD_ADD_ASSOC,word_add_n2w]
-  THEN1 (Cases_on `i'` \\ fs [inst_def,upd_pc_def]
-    \\ full_simp_tac std_ss [GSYM WORD_ADD_ASSOC,word_add_n2w])
-  \\ fs [jump_to_offset_def,upd_pc_def]
-  \\ full_simp_tac std_ss [GSYM WORD_ADD_ASSOC,word_add_n2w]);
 
 val _ = export_theory();
